Proof of red_tr fixed.

Semantics.v
@@ -256,12 +256,16 @@ Inductive redbinop : binop -> val -> val -> val -> Prop :=
       redbinop binop_add (val_int n1) (val_int n2) (val_int (n1 + n2))
   | redbinop_sub : forall n1 n2,
       redbinop binop_sub (val_int n1) (val_int n2) (val_int (n1 - n2))
-  | redbinop_eq : forall v1 v2,
+  | redbinop_eq_true : forall v1 v2,
       ~ is_error v1 ->
       ~ is_error v2 ->
-      redbinop binop_eq v1 v2 (val_bool (isTrue (v1 = v2))).
-
-Search empty.
+      v1 = v2 ->
+      redbinop binop_eq v1 v2 (val_bool true)
+  | redbinop_eq_false : forall v1 v2,
+      ~ is_error v1 ->
+      ~ is_error v2 ->
+      v1 <> v2 ->
+      redbinop binop_eq v1 v2 (val_bool false).
 
 
 (* ---------------------------------------------------------------------- *)
